refactor is now done. finished proving that the compiler does not change the semantics of the code. now just need to prove that the last stage has what is needed to stitch together the facts.

elle/ElleCorrect/Valid3.thy
@@ -173,6 +173,41 @@ proof(induction rule: ll_valid_q_ll_validl_q.induct)
     done
 qed
 
+lemma ll3_init_same' :
+"((! t' . ll3_init t = t' \<longrightarrow>
+  ll_purge_annot t' = ll_purge_annot t)
+\<and>
+(! ts' . map ll3_init ts = ts' \<longrightarrow>
+  map ll_purge_annot ts' = map ll_purge_annot ts))"
+proof(induction rule:my_ll_induct)
+case (1 q e i)
+then show ?case by auto
+next
+  case (2 q e idx)
+  then show ?case by auto
+next
+  case (3 q e idx n)
+  then show ?case by auto
+next
+  case (4 q e idx n)
+  then show ?case by auto
+next
+  case (5 q e l)
+  then show ?case by auto
+next
+  case 6
+  then show ?case by auto
+next
+  case (7 h l)
+  then show ?case by auto
+qed
+
+lemma ll3_init_same [rule_format] :
+"(! t' . ll3_init t = t' \<longrightarrow>
+  ll_purge_annot t' = ll_purge_annot t)"
+  apply(insert ll3_init_same') apply(blast)
+  done
+
 lemma ll3_consume_label_qvalid' :
 "((q, t) \<in> ll_valid_q \<longrightarrow> (! ls e . t = (LSeq e ls) \<longrightarrow> (! p p' n ls' . ll3_consume_label p n ls = Some (ls', p') \<longrightarrow> (q, LSeq e ls') \<in> ll_valid_q)))
 \<and> (((x,x'), ls) \<in> ll_validl_q \<longrightarrow> (! p p' n ls' . ll3_consume_label p n ls = Some (ls', p') \<longrightarrow> ((x,x'), ls') \<in> ll_validl_q ))"
@@ -572,6 +607,60 @@ lemma ll3_consume_none_gen :
   apply(blast+)
   done
 
+(* TODO: ll3_consume_label_same *)
+(* first case: map purge annot over the list and the list', assert equality *)
+(* better first case: assert that any Seq node resulting would be annotation-equal to original? Seems
+like unnecessary work *)
+(* second case: also map purge annot *)
+lemma ll3_consume_label_same' :
+  "(! e l q . (t :: ll3) = (q, LSeq e l) \<longrightarrow> (! p n p' l' . ll3_consume_label p n l = Some (l',p') \<longrightarrow>
+               map ll_purge_annot l = map ll_purge_annot l')) \<and>
+  (! l' p p' n . ll3_consume_label p n (l :: ll3 list) = Some (l', p') \<longrightarrow> map ll_purge_annot l = map ll_purge_annot l')"
+proof(induction rule:my_ll_induct)
+  case (1 q e i)
+  then show ?case by auto
+next
+  case (2 q e idx)
+  then show ?case by auto
+next
+  case (3 q e idx n)
+  then show ?case by auto
+next
+  case (4 q e idx n)
+  then show ?case by auto
+next
+  case (5 q e l)
+  then show ?case by auto
+next
+case 6
+  then show ?case by auto
+next
+case (7 h l)
+  then show ?case 
+    apply(auto)
+    apply(case_tac h, auto)
+    apply(case_tac ba, auto)
+         apply(case_tac "ll3_consume_label p (Suc n) l", auto)
+         apply(drule_tac x = aa in spec, auto)
+        apply(case_tac "x22 = length p", auto)
+         apply(case_tac "\<not> x21", auto)
+         apply(case_tac "ll3_consume_label p (Suc n) l", auto)
+         apply(drule_tac x = aa in spec, auto)
+         apply(case_tac "ll3_consume_label p (Suc n) l", auto)
+         apply(drule_tac x = aa in spec, auto)
+         apply(case_tac "ll3_consume_label p (Suc n) l", auto)
+      apply(drule_tac x = aa in spec, auto)
+     apply(case_tac "ll3_consume_label (n # p) 0 x52", auto)
+     apply(case_tac ba, auto)
+         apply(case_tac "ll3_consume_label p (Suc n) l", auto)
+    apply(drule_tac x = ab in spec, auto)
+    done
+qed
+
+lemma ll3_consume_label_same [rule_format]:
+"(! l' p p' n . ll3_consume_label p n (l :: ll3 list) = Some (l', p') \<longrightarrow> map ll_purge_annot l = map ll_purge_annot l')"
+  apply(insert ll3_consume_label_same') apply(blast)
+  done
 
 (* this statement isn't quite right *)
 (* need to generalize each side more? *)
@@ -713,6 +802,234 @@ lemma ll3_consumes_alt_eq_r2l2 [rule_format] :
   apply(case_tac x, auto)
   apply(drule_tac ll3_consumes_alt_eq_r2l)
   apply(auto simp add:ll3_consumes_alt.intros)
+  done
+
+inductive ll_purge_eq ::
+  "('lix, 'llx, 'ljx, 'ljix, 'lsx, 'ptx, 'pnx) ll \<Rightarrow>
+   ('li2x, 'll2x, 'lj2x, 'lji2x, 'ls2x, 'pt2x, 'pn2x) ll \<Rightarrow>
+  bool"
+  where
+"\<And> (t1 :: ('lix, 'llx, 'ljx, 'ljix, 'lsx, 'ptx, 'pnx) ll)
+    (t2 :: ('li2x, 'll2x, 'lj2x, 'lji2x, 'ls2x, 'pt2x, 'pn2x) ll)
+ . (ll_purge_annot t1) = (ll_purge_annot t2) \<Longrightarrow>
+  ll_purge_eq t1 t2"
+
+lemma ll_purge_eq_trans [rule_format] :
+  "ll_purge_eq t1 t2 \<Longrightarrow>
+   (! t3 . ll_purge_eq t2 t3 \<longrightarrow> ll_purge_eq t1 t3)"
+proof(induction rule:ll_purge_eq.induct)
+  case (1 t1 t2)
+  then show ?case
+    apply(auto)
+    apply(drule_tac ll_purge_eq.cases) apply(auto)
+    apply(rule_tac ll_purge_eq.intros) apply(auto)
+    done
+qed
+
+lemma ll_purge_eq_refl :
+  "ll_purge_eq t t"
+  apply(auto simp add:ll_purge_eq.intros)
+  done
+
+lemma ll_purge_eq_sym [rule_format] :
+  "ll_purge_eq t1 t2 \<Longrightarrow> ll_purge_eq t2 t1"
+proof(induction rule:ll_purge_eq.induct)
+  case (1 t1 t2)
+  then show ?case
+    apply(rule_tac ll_purge_eq.intros)
+    apply(auto)
+    done
+qed
+  
+
+inductive ll_purge_eqs ::
+  "('lix, 'llx, 'ljx, 'ljix, 'lsx, 'ptx, 'pnx) ll list \<Rightarrow>
+   ('li2x, 'll2x, 'lj2x, 'lji2x, 'ls2x, 'pt2x, 'pn2x) ll list \<Rightarrow>
+  bool"
+  where
+"\<And> (l1 :: ('lix, 'llx, 'ljx, 'ljix, 'lsx, 'ptx, 'pnx) ll list)
+    (l2 :: ('li2x, 'll2x, 'lj2x, 'lji2x, 'ls2x, 'pt2x, 'pn2x) ll list)
+ . (map ll_purge_annot l1) = (map ll_purge_annot l2) \<Longrightarrow>
+  ll_purge_eqs l1 l2"
+
+lemma ll_purge_eqs_trans [rule_format] :
+  "ll_purge_eqs t1 t2 \<Longrightarrow>
+   (! t3 . ll_purge_eqs t2 t3 \<longrightarrow> ll_purge_eqs t1 t3)"
+proof(induction rule:ll_purge_eqs.induct)
+  case (1 t1 t2)
+  then show ?case
+    apply(auto)
+    apply(drule_tac ll_purge_eqs.cases) apply(auto)
+    apply(rule_tac ll_purge_eqs.intros) apply(auto)
+    done
+qed
+
+lemma ll_purge_eqs_refl :
+  "ll_purge_eqs t t"
+  apply(auto simp add:ll_purge_eqs.intros)
+  done
+
+lemma ll_purge_eqs_sym [rule_format] :
+  "ll_purge_eqs t1 t2 \<Longrightarrow> ll_purge_eqs t2 t1"
+proof(induction rule:ll_purge_eqs.induct)
+  case (1 t1 t2)
+  then show ?case
+    apply(rule_tac ll_purge_eqs.intros)
+    apply(auto)
+    done
+qed
+
+lemma ll_purge_eq_seq [rule_format] :
+  "ll_purge_eq t1 t2 \<Longrightarrow>
+    (! q1 e1 l1 . t1 = (q1, LSeq e1 l1) \<longrightarrow>
+    (? q2 e2 l2 . t2 = (q2, LSeq e2 l2) \<and>
+    ll_purge_eqs l1 l2))"
+proof(induction rule:ll_purge_eq.induct)
+  case (1 t1 t2)
+  then show ?case
+    apply(auto)
+    apply(case_tac t2, auto) apply(case_tac baa, auto)
+    apply(rule_tac ll_purge_eqs.intros) apply(auto)
+    done
+qed
+
+lemma ll_purge_eqs_seq [rule_format] :
+  "ll_purge_eqs l1 l2 \<Longrightarrow>
+   (! q1 e1 q2 e2 .
+    ll_purge_eq (q1, LSeq e1 l1) (q2, LSeq e2 l2))"
+proof(induction rule:ll_purge_eqs.induct)
+  case (1 l1 l2)
+  then show ?case
+    apply(auto)
+    apply(rule_tac ll_purge_eq.intros)
+    apply(auto)
+    done
+qed
+
+
+
+(* ugh... let's create a new relation to guide the simplifier then *)
+(* need an extra generalization about how we are running on not just our l,
+but on any ll3 that has the same purge_annotations as our original list
+do we need this in the second branch or just first? *)
+(* idea: ll_purge_eq t t2 *)
+lemma ll3_assign_label_same' :
+"(! t2 . ll_purge_eq (t :: ll3) (t2 :: ll3) \<longrightarrow>
+  (! q' t' .  ll3_assign_label t2  = Some t' \<longrightarrow> ll_purge_eq t t')) \<and>
+ ( ! l2. ll_purge_eqs (l :: ll3 list) (l2 :: ll3 list) \<longrightarrow>
+  (! l' . ll3_assign_label_list (l2 :: ll3 list) = Some l' \<longrightarrow> 
+      ll_purge_eqs l l'))"
+proof(induction rule:my_ll_induct)
+case (1 q e i)
+  then show ?case 
+    apply(auto)
+    apply(case_tac ba, auto)
+     apply(drule_tac ll_purge_eq.cases)
+      apply(auto)
+     apply(drule_tac ll_purge_eq.cases, auto)
+    done
+next
+  case (2 q e idx)
+  then show ?case 
+    apply(auto)
+    apply(case_tac ba, auto)
+     apply(case_tac x21, auto)
+     apply(drule_tac ll_purge_eq.cases, auto)
+    done
+next
+  case (3 q e idx n)
+  then show ?case
+    apply(auto)
+    apply(case_tac ba, auto)
+     apply(drule_tac ll_purge_eq.cases, auto)
+     apply(drule_tac ll_purge_eq.cases, auto)
+    done
+next
+  case (4 q e idx n)
+  then show ?case
+    apply(auto)
+    apply(case_tac ba, auto)
+     apply(drule_tac ll_purge_eq.cases, auto)
+     apply(drule_tac ll_purge_eq.cases, auto)
+    done
+next
+  case (5 q e l)
+  then show ?case 
+    apply(clarify)
+    apply(auto)
+    apply(case_tac ba, auto)
+     apply(drule_tac ll_purge_eq_seq, auto)
+apply(drule_tac ll_purge_eq_seq, auto)
+    apply(case_tac "ll3_consume_label [] 0 x52", auto)
+    apply(rename_tac boo) 
+    apply(case_tac "ll3_assign_label_list ab", auto)
+(* need consume eq here *)
+    apply(frule_tac ll3_consume_label_same)
+    apply(drule_tac ll_purge_eqs.intros)
+    apply(drule_tac x = ab in spec)
+    apply(drule_tac ll_purge_eqs_trans)
+     apply(auto)
+    apply(rule_tac ll_purge_eqs_seq) apply(auto)
+    done
+next
+  case 6
+  then show ?case 
+    apply(auto)
+    apply(case_tac l2, auto)
+    apply(drule_tac ll_purge_eqs.cases, auto)
+    done
+next
+  case (7 h l)
+  then show ?case 
+    apply(clarify)
+    apply(case_tac l2, auto)
+    apply(case_tac "ll3_assign_label ((a, b), ba)", auto)
+    apply(case_tac "ll3_assign_label_list list", auto)
+    apply(drule_tac ll_purge_eqs.cases, auto)
+    apply(rule_tac ll_purge_eqs.intros, auto)
+
+     apply(drule_tac ll_purge_eq.intros)
+    apply(drule_tac x = a in spec, rotate_tac -1)
+    apply(drule_tac x = b in spec, rotate_tac -1)
+     apply(drule_tac x = ba in spec, rotate_tac -1) apply(auto)
+    apply(rotate_tac -1)
+     apply(drule_tac ll_purge_eq_sym) apply(rotate_tac -1)
+apply(drule_tac ll_purge_eq_trans)  apply(auto)
+     apply(drule_tac ll_purge_eq.cases) apply(auto)
+     apply(drule_tac ll_purge_eq.cases, auto)
+
+    apply(rotate_tac 1)
+    apply(drule_tac x = list in spec)
+    apply(drule_tac ll_purge_eqs.intros)
+    apply(auto)
+    apply(rotate_tac -1)
+    apply(drule_tac ll_purge_eqs_sym, rotate_tac -1)
+    apply(drule_tac ll_purge_eqs_trans, auto)
+    apply(rotate_tac -1)
+    apply(drule_tac ll_purge_eqs.cases)
+    apply(auto)
+    done
+qed
+(*
+(! t2 . ll_purge_eq (t :: ll3) (t2 :: ll3) \<longrightarrow>
+  (! q' t' .  ll3_assign_label t2  = Some t' \<longrightarrow> ll_purge_eq t t')
+*)
+
+lemma ll3_assign_label_same'2 [rule_format] :
+"(! t2 . ll_purge_eq (t :: ll3) (t2 :: ll3) \<longrightarrow>
+  (! q' t' .  ll3_assign_label t2  = Some t' \<longrightarrow> ll_purge_eq t t'))"
+  apply(insert ll3_assign_label_same')  apply(auto)
+  done
+
+
+lemma ll3_assign_label_same [rule_format] :
+"ll3_assign_label t  = Some t' \<Longrightarrow> ll_purge_annot t = ll_purge_annot t'"
+  apply(insert ll3_assign_label_same'2[of t t t'])
+  apply(auto)
+  apply(subgoal_tac "ll_purge_eq t t")
+   apply(rule_tac[2] ll_purge_eq_refl)
+  apply(auto)
+  apply(drule_tac ll_purge_eq.cases) apply(auto)
   done
 
 (* building up to assign label q valid proof *)
